src/tls/TLSError.fst
@@ -67,5 +67,31 @@ type error = alertDescription * string
 
 type Result 'a = Platform.Error.optResult error 'a
 
+open Platform.Error
+
 val resT: r:Result 'a { Platform.Error.is_Correct r } -> Tot 'a
 let resT (Platform.Error.Correct v) = v
+
+val mapResult: ('a -> Tot 'b) -> Result 'a -> Tot (Result 'b)
+let mapResult f r = 
+   (match r with
+    | Error z -> Error z
+    | Correct c -> Correct (f c))
+
+val bindResult: ('a -> Tot (Result 'b)) -> Result 'a -> Tot (Result 'b)
+let bindResult f r = 
+   (match r with
+    | Error z -> Error z
+    | Correct c -> f c)
+
+val resultMap: Result 'a -> ('a -> Tot 'b) -> Tot (Result 'b)
+let resultMap r f = 
+   (match r with
+    | Error z -> Error z
+    | Correct c -> Correct (f c))
+
+val resultBind: Result 'a -> ('a -> Tot (Result 'b)) -> Tot (Result 'b)
+let resultBind r f = 
+   (match r with
+    | Error z -> Error z
+    | Correct c -> f c)
