src/tls/HASH.fst
@@ -11,6 +11,7 @@ open TLSConstants
 
 (* Parametric hash algorithm (implements interface) *)
 // FIXME: had to add a type annotation to make this go through
+val hash': hashAlg -> bytes -> Tot bytes
 let hash' alg data: bytes =
     match alg with
     | NULL    -> data
@@ -18,9 +19,13 @@ let hash' alg data: bytes =
     | Hash h  -> (CoreCrypto.hash h  data)
 
 // FIXME: same here
+val hash: hashAlg -> bytes -> Tot bytes
 let hash alg data: bytes =
   let h = hash' alg data in
   let l = length h in
+    h
+(*
   let exp = hashSize alg in
   if l = exp then h
   else Platform.Error.unexpected "CoreCrypto.Hash returned a hash of an unexpected size"
+*)
